\documentclass{article}

\usepackage{amsmath,esint}

\newcommand*\VF[1]{\mathbf{#1}}
\newcommand*\dif{\mathop{}\!\mathrm{d}}

\begin{document}

\begin{align*}
  \iiint\limits_V (\nabla \cdot \VF{F}) \dif V
  &= \oiint\limits_{S(V)} \VF{F} \cdot \hat{\VF{n}} \dif S\\
  \iiint\limits_V (\nabla \times \VF{F}) \dif V
  &= \oiint \hat{\VF{n}} \times \VF{F} \dif S
\end{align*}





\begin{align*}
  \iiint_{V} (\nabla \cdot \VF{F}) \dif V
  &= \oiint_{S(V)} \VF{F} \cdot \hat{\VF{n}} \dif S\\
  \iiint_{V} (\nabla \times \VF{F}) \dif V
  &= \oiint \hat{\VF{n}} \times \VF{F} \dif S
\end{align*}


\begin{align*}
  \iiint\limits_V(\nabla \cdot \mathbf{F}) dV
      & = \oiint \limits_{S(V)} \mathbf{F \cdot \hat{n}} dS \\
  \iiint\limits_V(\nabla \times \mathbf{F}) dV
      & = \oiint \limits_{S(V)} \mathbf{\hat{n} \times F} dS \\
  \iiint\limits_V(\nabla f) dV
      & = \oiint\limits_{S(V)}\mathbf{\hat{n}}f dS
\end{align*}


\end{document}